library/init/meta/converter/interactive.lean
@@ -39,7 +39,7 @@ conv.skip
 meta def whnf : conv unit :=
 conv.whnf
 
-meta def dsimp (no_dflt : parse only_flag) (es : parse opt_qexpr_list) (attr_names : parse with_ident_list)
+meta def dsimp (no_dflt : parse only_flag) (es : parse tactic.simp_arg_list) (attr_names : parse with_ident_list)
                (ids : parse without_ident_list) (cfg : tactic.dsimp_config := {}) : conv unit :=
 do (s, u) ← tactic.mk_simp_set no_dflt attr_names es ids,
    conv.dsimp (some s) u cfg
@@ -108,7 +108,7 @@ do (r, lhs, _) ← tactic.target_lhs_rhs,
        r lhs,
   update_lhs new_lhs pr
 
-meta def simp (no_dflt : parse only_flag) (hs : parse opt_qexpr_list) (attr_names : parse with_ident_list)
+meta def simp (no_dflt : parse only_flag) (hs : parse tactic.simp_arg_list) (attr_names : parse with_ident_list)
               (ids : parse without_ident_list) (cfg : tactic.simp_config_ext := {})
               : conv unit :=
 do (s, u) ← tactic.mk_simp_set no_dflt attr_names hs ids,
