library/data/list/comb.lean
@@ -91,7 +91,7 @@ theorem foldr_append (f : α → β → β) :
 | b (a::l₁) l₂ := by simp [foldr_append]
 
 theorem foldl_reverse (f : α → β → α) (a : α) (l : list β) : foldl f a (reverse l) = foldr (λx y, f y x) a l :=
-by induction l; simph [foldl, foldr]
+by induction l; simp [*, foldl, foldr]
 
 theorem foldr_reverse (f : α → β → β) (a : β) (l : list α) : foldr f a (reverse l) = foldl (λx y, f y x) a l :=
 let t := foldl_reverse (λx y, f y x) a (reverse l) in
